try making address of pointsto Z

examples/load_test.v
@@ -4,12 +4,12 @@ Require Import isla.instructions.instr_ldr.
 Definition spec `{!islaG Σ} `{!threadG} a : iProp Σ :=
   ∃ (vold : bv 64),
   "R1" ↦ᵣ RVal_Bits [BV{64} 0x0000000000000008] ∗
-  [BV{64} 0x0000000000000008] ↦ₘ [BV{64} 0x00000000deadbeef] ∗
+  0x0000000000000008 ↦ₘ [BV{64} 0x00000000deadbeef] ∗
   "R0" ↦ᵣ RVal_Bits vold ∗
   reg_col sys_regs ∗
   instr_pre a (
     "R1" ↦ᵣ RVal_Bits [BV{64} 0x0000000000000008] ∗
-    [BV{64} 0x0000000000000008] ↦ₘ [BV{64} 0x00000000deadbeef] ∗
+    0x0000000000000008 ↦ₘ [BV{64} 0x00000000deadbeef] ∗
     "R0" ↦ᵣ RVal_Bits [BV{64} 0x00000000deadbeef] ∗
     reg_col sys_regs ∗
     True).
