examples/store_test.v
@@ -3,12 +3,12 @@ Require Import isla.instructions.instr_str.
 
 Definition spec `{!islaG Σ} `{!threadG} a : iProp Σ :=
   "R1" ↦ᵣ RVal_Bits [BV{64} 0x0000000000000008] ∗
-  [BV{64} 0x0000000000000008] ↦ₘ [BV{64} 0x00000000deadbeef] ∗
+  0x0000000000000008 ↦ₘ [BV{64} 0x00000000deadbeef] ∗
   "R9" ↦ᵣ RVal_Bits [BV{64} 0x00000000cafebabe] ∗
   reg_col sys_regs ∗
   instr_pre a (
     "R1" ↦ᵣ RVal_Bits [BV{64} 0x0000000000000008] ∗
-    [BV{64} 0x0000000000000008] ↦ₘ [BV{64} 0x00000000cafebabe] ∗
+    0x0000000000000008 ↦ₘ [BV{64} 0x00000000cafebabe] ∗
     "R9" ↦ᵣ RVal_Bits [BV{64} 0x00000000cafebabe] ∗
     reg_col sys_regs ∗
     True).
