examples/stp_test.v
@@ -5,8 +5,8 @@ Definition spec `{!islaG Σ} `{!threadG} a sp (v1 v2 : bv 64) : iProp Σ :=
   ∃ (vold1 vold2 : bv 64),
   "R0" ↦ᵣ RVal_Bits v1 ∗
   "R1" ↦ᵣ RVal_Bits v2 ∗
-  (bv_sub sp [BV{64} 16]) ↦ₘ vold1 ∗
-  (bv_sub sp [BV{64} 8]) ↦ₘ vold2 ∗
+  (bv_unsigned sp - 16) ↦ₘ vold1 ∗
+  (bv_unsigned sp - 8) ↦ₘ vold2 ∗
   ⌜bv_unsigned sp `mod` 8 = 0⌝ ∗
   ⌜16 < bv_unsigned sp < 2 ^ 52⌝ ∗
   "SP_EL2" ↦ᵣ RVal_Bits sp ∗
@@ -16,8 +16,8 @@ Definition spec `{!islaG Σ} `{!threadG} a sp (v1 v2 : bv 64) : iProp Σ :=
     "R1" ↦ᵣ RVal_Bits v2 ∗
     "SP_EL2" ↦ᵣ RVal_Bits (bv_sub sp [BV{64} 16])∗
     reg_col sys_regs ∗
-    (bv_sub sp [BV{64} 16]) ↦ₘ v1 ∗
-    (bv_sub sp [BV{64} 8]) ↦ₘ v2 ∗
+    (bv_unsigned sp - 16) ↦ₘ v1 ∗
+    (bv_unsigned sp - 8) ↦ₘ v2 ∗
     True).
 
 Lemma stp_wp `{!islaG Σ} `{!threadG} (sp v1 v2: bv 64):
