examples/riscv64_test.v
@@ -21,7 +21,7 @@ Lemma riscv_test `{!islaG Σ} `{!threadG} (x2 x11 : bv 64):
     "x11" ↦ᵣ RVal_Bits x11 ∗
     ⌜bv_unsigned x2 `mod` 8 = 0⌝ ∗
     ⌜0x0000000080000000 ≤ bv_unsigned x2 + 8 < 0x0000000080000000 + 0x0000000004000000⌝ ∗
-    bv_add_Z x2 8 ↦ₘ? 8 ∗
+    (bv_unsigned x2 + 8) ↦ₘ? 8 ∗
     spec_trace (riscv_test_spec x11) ∗
     True
   ).
@@ -57,34 +57,37 @@ Local Arguments list_to_map : simpl never.
 Lemma riscv_test_adequate mstatus_bits satp x2 x10 x11 κs n t2 σ2:
   bv_extract 17 1 mstatus_bits = [BV{1} 0] →
   bv_unsigned x2 `mod` 8 = 0 →
+  bv_unsigned x2 + 16 < 2 ^ 64 →
   0x0000000080000000 ≤ bv_unsigned x2 + 8 < 0x0000000080000000 + 0x0000000004000000 →
   nsteps n (initial_local_state <$> [riscv_test_regs mstatus_bits satp x2 x10 x11],
             riscv_test_state_global x2) κs (t2, σ2) →
   (∀ e2, e2 ∈ t2 → not_stuck e2 σ2) ∧ riscv_test_spec x11 κs.
 Proof.
-  move => ???.
+  move => ????.
   set Σ : gFunctors := #[islaΣ].
   apply: (isla_adequacy Σ) => //.
   { unfold riscv_test_spec. destruct (decide ((bv_unsigned x11 = 1))); spec_solver. }
   iIntros (?) "#Hi #Hbm Hspec Hmem /= !>". iSplitL => //. iIntros (?).
-  iAssert (bv_add_Z x2 8 ↦ₘ? 8)%I with "[Hmem]" as "?". {
+  iAssert ((bv_unsigned x2 + 8) ↦ₘ? 8)%I with "[Hmem]" as "?". {
     rewrite big_sepM_list_to_map. 2: { rewrite fst_zip //. by apply NoDup_bv_seq. }
-    rewrite /zip_with/=.
+    rewrite /zip_with/=. iClear "Hbm".
     iDestruct "Hmem" as "(Hm1&Hm2&Hm3&Hm4&Hm5&Hm6&Hm7&Hm8&_)".
-    rewrite bv_add_Z_0.
+    rewrite bv_add_Z_0 -!bv_add_Z_add_r !bv_add_Z_unsigned !bv_wrap_small; [|bv_solve..].
+    rewrite -!Z.add_assoc.
     iApply (mem_mapsto_uninit_combine 1 with "[Hm1]"); [done|by iApply (mem_mapsto_mapsto_to_uninit _ _ 8)|].
+    rewrite -!Z.add_assoc.
     iApply (mem_mapsto_uninit_combine 1 with "[Hm2]"); [done|by iApply (mem_mapsto_mapsto_to_uninit _ _ 8)|].
-    rewrite -(bv_add_Z_add_r _ 1 1).
+    rewrite -!Z.add_assoc.
     iApply (mem_mapsto_uninit_combine 1 with "[Hm3]"); [done|by iApply (mem_mapsto_mapsto_to_uninit _ _ 8)|].
-    rewrite -(bv_add_Z_add_r _ 1 _).
+    rewrite -!Z.add_assoc.
     iApply (mem_mapsto_uninit_combine 1 with "[Hm4]"); [done|by iApply (mem_mapsto_mapsto_to_uninit _ _ 8)|].
-    rewrite -(bv_add_Z_add_r _ 1 _).
+    rewrite -!Z.add_assoc.
     iApply (mem_mapsto_uninit_combine 1 with "[Hm5]"); [done|by iApply (mem_mapsto_mapsto_to_uninit _ _ 8)|].
-    rewrite -(bv_add_Z_add_r _ 1 _).
+    rewrite -!Z.add_assoc.
     iApply (mem_mapsto_uninit_combine 1 with "[Hm6]"); [done|by iApply (mem_mapsto_mapsto_to_uninit _ _ 8)|].
-    rewrite -(bv_add_Z_add_r _ 1 _).
+    rewrite -!Z.add_assoc.
     iApply (mem_mapsto_uninit_combine 1 with "[Hm7]"); [done|by iApply (mem_mapsto_mapsto_to_uninit _ _ 8)|].
-    rewrite -(bv_add_Z_add_r _ 1 _).
+    rewrite -!Z.add_assoc.
     iApply (mem_mapsto_uninit_combine 1 with "[Hm8]"); [done|by iApply (mem_mapsto_mapsto_to_uninit _ _ 8)|].
     by rewrite mem_mapsto_uninit_0.
   }
