theories/riscv64/specs.v
@@ -7,14 +7,14 @@ Definition sd_spec `{!islaG Σ} `{!threadG} (pc : Z) (R1 R2 : string) (offset : 
   reg_col sys_regs ∗
   R1 ↦ᵣ RVal_Bits r1 ∗
   R2 ↦ᵣ RVal_Bits r2 ∗
-  (bv_add_Z r2 offset) ↦ₘ? 8 ∗
+  (bv_unsigned r2 + offset) ↦ₘ? 8 ∗
   ⌜bv_unsigned r2 `mod` 8 = 0⌝ ∗
   ⌜0x0000000080000000 ≤ bv_unsigned r2 + offset < 0x0000000080000000 + 0x0000000004000000⌝ ∗
   instr_pre (pc + 4) (
     reg_col sys_regs ∗
     R1 ↦ᵣ RVal_Bits r1 ∗
     R2 ↦ᵣ RVal_Bits r2 ∗
-    (bv_add_Z r2 offset) ↦ₘ r1 ∗
+    (bv_unsigned r2 + offset) ↦ₘ r1 ∗
     True
   ).
 Global Instance : LithiumUnfold (@sd_spec) := I.
@@ -24,14 +24,14 @@ Definition ld_spec `{!islaG Σ} `{!threadG} (pc : Z) (R1 R2 : string) (offset : 
   reg_col sys_regs ∗
   R1 ↦ᵣ: λ _,
   R2 ↦ᵣ RVal_Bits r2 ∗
-  (bv_add_Z r2 offset) ↦ₘ r1 ∗
+  (bv_unsigned r2 + offset) ↦ₘ r1 ∗
   ⌜bv_unsigned r2 `mod` 8 = 0⌝ ∗
   ⌜0x0000000080000000 ≤ bv_unsigned r2 + offset < 0x0000000080000000 + 0x0000000004000000⌝ ∗
   instr_pre (pc + 4) (
     reg_col sys_regs ∗
     R1 ↦ᵣ RVal_Bits r1 ∗
     R2 ↦ᵣ RVal_Bits r2 ∗
-    (bv_add_Z r2 offset) ↦ₘ r1 ∗
+    (bv_unsigned r2 + offset) ↦ₘ r1 ∗
     True
   ).
 Global Instance : LithiumUnfold (@ld_spec) := I.
